Added notation and used Focus for more clarity (despite its being deprecated...)

lab5/extra/demo-factorial.v
@@ -1,20 +1,21 @@
 Require Import Arith.
+Import Nat.
 
 
-Load hoare.
+Load "./hoare".
 
 
-  (* From "Formal Reasoning About Programs"
+(* From "Formal Reasoning About Programs"
 
-     factorial(n) {
-        a = 1;
-        while (n > 0) {
-           a = a * n;
-           n = n - 1;
-        }
-        return a; 
-     }
-  *)
+   factorial(n) {
+      a = 1;
+      while (n > 0) {
+         a = a * n;
+         n = n - 1;
+      }
+      return a; 
+   }
+*)
 
 Definition gt01 n m := if gt_dec n m then 1 else 0.
 
@@ -22,25 +23,29 @@ Notation "[ e1 `*` e2 ]" := (expr_op e1 mul e2).
 Notation "[ e1 `-` e2 ]" := (expr_op e1 sub e2).
 Notation "[ e1 `>` e2 ]" := (expr_op e1 gt01 e2).
 
+Notation "$ v" := (expr_var v) (at level 7, format "$ v").
+Notation "# n" := (expr_num n) (at level 7, format "# n").
+
+
 Definition factorial_cmd :=
-  seq (assign a (expr_num 1))
-      (while [expr_var n `>` expr_num 0]
-             (seq (assign a [expr_var a `*` expr_var n])
-                  (assign n [expr_var n `-` expr_num 1]))).
+  seq (assign a (#1))
+      (while [$n `>` #0]
+             (seq (assign a [$a `*` $n])
+                  (assign n [$n `-` #1]))).
 
 
 
 Module MainProof.
 
-  Definition c := seq (assign a [expr_var a `*` expr_var n])
-                      (assign n [expr_var n `-` expr_num 1]).
+  Definition c := seq (assign a [$a `*` $n])
+                      (assign n [$n `-` $1]).
 
-  Definition linv n0 s := s a * fact (s n) = fact n0.
+  Definition linv n0 (s : state) := s a * fact (s n) = fact n0.
 
   (* Control the behavior of `simpl` to allow more unfoldings.            *)
   (*                                                                      *)
   (* This should allow you to simplify a substitution term,               *)
-  (*   e.g. subst (fun s => s a + 1 = 2) a [expr_var a `-` expr_num 1] s  *)
+  (*   e.g. subst (fun s => s a + 1 = 2) a [$a `-` #1] s                  *)
   (*        ( in other words, (a + 1 = 2)[a - 1 / a] )                    *)
   (*     simplifies to                                                    *)
   (*        s a - 1 + 1 = 2                                               *)
@@ -53,13 +58,13 @@ Module MainProof.
                                  c
                                  (linv n0).
   Proof.
-    unfold c. econstructor.
-    2: constructor.     (* abrrev. for `Focus 2. constructor.` *)
-    simpl. unfold linv; simpl.
-    eapply hoare_weaken_l. 
-    2: constructor.
+    unfold c. unfold linv. eapply hoare_seq.
+    Focus 2. apply hoare_assign.
     simpl.
-    intros. firstorder.
+    eapply hoare_weaken_l.
+    Focus 2. apply hoare_assign.
+    simpl.
+    firstorder.
     destruct (s n) as [|k].
     - inversion H0.
     - simpl.
@@ -99,5 +104,6 @@ Module MainProof.
   Qed.
 
 End MainProof.
+
 
 
