lab5/src/euclid.v
@@ -22,6 +22,9 @@ Notation "[ e1 `-` e2 ]" := (expr_op e1 sub e2).
 Notation "[ e1 `>` e2 ]" := (expr_op e1 gt01 e2).
 Notation "[ e1 `!=` e2 ]" := (expr_op e1 ne01 e2).
 
+Notation "$ v" := (expr_var v) (at level 7, format "$ v").
+Notation "# n" := (expr_num n) (at level 7, format "# n").
+
 
 Definition euclid_cmd :=
   while [expr_var a `!=` expr_var b]
@@ -37,8 +40,9 @@ Notation "( a | b )" := (divides a b).
 
 
 (* Control the behavior of `simpl` to allow more unfoldings.            *)
+(*                                                                      *)
 (* This should allow you to simplify a substitution term,               *)
-(*   e.g. subst (fun s => s a + 1 = 2) a [expr_var a `-` expr_num 1] s  *)
+(*   e.g. subst (fun s => s a + 1 = 2) a [$a `-` #1] s                  *)
 (*        ( in other words, (a + 1 = 2)[a - 1 / a] )                    *)
 (*     simplifies to                                                    *)
 (*        s a - 1 + 1 = 2                                               *)
